Square Root Theory
================

This theory originated when I was 12 years old in school. Over time, it has evolved into a concept with a mathematical explanation. Initially designed to find the square root of a number without relying on the square root function, it also extends to the calculation of the square of a number. The function I devised is represented as follows:

$$ f(x) = 2 a + b-1 $$
$$ a \in A $$
$$ b \in B $$

Where: 

$$ A = {a \in \mathbb{N}} $$

$$ B = {b \in \mathbb{N}} $$

$$ \mathbb{N} = {0, 1, 2, 3, 4, 5, 6, 7, 8, 9, ...\} $$

$$ a_0 = 1 $$

$$ b_0 = 0 $$

Summary: Vector-Based Square Root Approach

In summary, Vector A represents a sequence of numbers denoted as 'a,' ranging from 1 to X, while Vector B encapsulates a series of corresponding values 'b,' spanning from 0 to the square of X. The distinguishing feature of this approach lies in its independence from the square root function, rendering it highly adaptable for implementation in various programming languages.

It is crucial to acknowledge that, while this function exhibits exceptional performance with natural numbers possessing an exact square root, it extends its utility to any scenario where determining the square of a number is the primary objective. The inherent flexibility and programming-friendly nature of this method make it a valuable alternative for computational tasks, contributing a unique perspective to numerical calculations.

The algorithm is as follows:
```
Function Equation(a, b)
    Return (b + 2 * a - 1)
```
This explanation is simplified as the function starts with a=1 and b=0. The rationale behind this lies in the fact that b represents the square of a-1, and a begins with 1 since the square of 0 is 0, and the square of 1 is 1. The function is essentially the sum of b-1 plus two times a. This formulation stems from my observation in youth that the difference between the square of a number and the square of the next number is consistently the next odd number. For instance, the difference between the square of 1 and the square of 2 is 3, and similarly, the difference between the square of 2 and the square of 3 is 5. Therefore, the function embodies the sum of the previous square plus the next odd number, revealing an intriguing pattern discovered in early explorations of numerical sequences.

Imagine that: A is a line with natural numbers, B is a line with this numbers squared and C is a line that represents the number that need to be sumed to the previous square to get the next square.

A = {1, 2, 3, 4, 5, 6, 7, 8, 9, 10, ...}

B = {0, 1, 4, 9, 16, 25, 36, 49, 64, 81, ...}

C = {1, 3, 5, 7, 9, 11, 13, 15, 17, 19, ...}

The function, therefore, manifests as the sum of the preceding square and the subsequent odd number. This was a concept I conceived years ago, and I'm genuinely intrigued to ascertain if there exists a theorem or any formal recognition of this pattern. It is genuinely fascinating. I am delighted to share this with you, even if there is an existing theorem related to it. This idea originated when I was 12 years old, and I take pride in having explored such concepts at a young age.

Appreciate your reading! The code resides in this repository, and I've implemented it in Python, as it's the language I'm currently predominantly using. If you wish to employ it in another language, feel free to translate the code; it's a straightforward process. Enjoy! :)


